Verification

verification_finalised/Exopire/expire.dfy
@@ -1,4 +1,27 @@
-   method Remove(key:int) returns (newValues:seq<int>)
+class Dynamic_array{
+   var values: seq<int>;
+   predicate Valid()
+   reads this;
+   {
+      |values|>=0
+   }
+   constructor ()
+   modifies this;
+   ensures Valid();
+   ensures |values|==0;
+   {
+      values:=[];
+   }
+   
+   method Length() returns (num:int)
+   requires Valid();
+   ensures Valid();
+   ensures num==|values|
+   {
+      num:=|values|;
+   }
+   
+   method Remove(key:int)
    requires Valid();
    ensures Valid();
    ensures (forall k::0<=k<|old(values)| && k !=key ==> old(values)[k] in values);
@@ -13,29 +36,273 @@
       assert(forall k::0<=k<|old(values)| && k !=key ==> old(values)[k] in values);
       
    }
+   
+   
+   
+   method Add(key:int,value:int)
+   requires Valid();
+   requires 0<=key<=|values|
+   ensures Valid();
+   ensures |values|==|old(values)|+1;
+   ensures (values[key]==value);
+   ensures (forall k:: 0<=k<|old(values)| ==> old(values)[k] in values);
+   ensures (forall k:: (k in values <==> k in old(values) || k==value ));
+   ensures (forall k:: (!( k in old(values) || k==value )) ==>(! (k in values)));
+   modifies this;
+   {
+      var tmp_seq:=[value];
+      assert(|tmp_seq|==1);
+      var newValues := values[..key]+tmp_seq[0..|tmp_seq|]+values[key..|values|];
+      assert(|newValues|==|values|+1);
+      assert(0<=key<|newValues|);
+      assert(newValues[key]==value);
+      assert(forall k:: 0<=k<|values| ==> values[k] in newValues);
+      values:=newValues;
+   }
+   
+   
+   
+   method Change(newValues: seq<int>)
+   requires Valid();
+   ensures Valid();
+   modifies this;
+   {
+      values:=newValues;
+   }
+   
 
+}
 
-
-method discard_by_id (bloodArray: array?<int>, id: int) returns (result:bool)
+method discard_by_id (bloodArray: Dynamic_array, id: int) returns (result:bool)
     requires bloodArray!=null && !(id<0);
     //All ids need to be unique
-    requires forall k,i:: 0<=k<i<bloodArray.Length ==> bloodArray[i] != bloodArray[k]
+    requires forall k,i:: 0<=k<i< |bloodArray.values| ==> bloodArray.values[i] != bloodArray.values[k]
     requires id >= 0;
-    ensures result==true ==> (exists k:: 0<=k<bloodArray.Length && bloodArray[k]==id)
+    ensures result==true ==> (exists k:: 0<=k< old(|bloodArray.values|) && old(bloodArray.values[k]==id))
+    modifies bloodArray;
 {
     var i := 0;
     result := false;
-    while (i<bloodArray.Length)
-    invariant 0<=i<=bloodArray.Length;
-    invariant result ==true ==> forall k:: 0<=k<bloodArray.Length ==> bloodArray[k]!=id
+    while (i< |bloodArray.values|)
+    invariant 0<=i<= |bloodArray.values|;
+    invariant result ==true ==> forall k:: 0<=k< |bloodArray.values| ==> bloodArray.values[k]!=id
     {
-        if (bloodArray[i] == id){
+        if (bloodArray.values[i] == id){
+            assert(bloodArray.values[i] == id);
             result:= true;
-            return result;
+            bloodArray.Remove(i);
+            return;
         }else{
             result:= false;
         }
         i:=i+1;
     }
-    return result;
+    return;
+}
+
+ this;
+   ensures Valid();
+   ensures |values|==0;
+   {
+      values:=[];
+   }
+   
+   method Length() returns (num:int)
+   requires Valid();
+   ensures Valid();
+   ensures num==|values|
+   {
+      num:=|values|;
+   }
+   
+   method Remove(key:int)
+   requires Valid();
+   ensures Valid();
+   ensures (forall k::0<=k<|old(values)| && k !=key ==> old(values)[k] in values);
+   modifies this;
+   {
+      if(key>=|values| || key <0 |||values|==0){
+         return;
+      }
+      assert(|values|>0&&|values|>key);
+      values := values[..key]+values[(key+1)..|values|];
+      assert(|values|+1==|old(values)|);
+      assert(forall k::0<=k<|old(values)| && k !=key ==> old(values)[k] in values);
+      
+   }
+   
+   
+   
+   method Add(key:int,value:int)
+   requires Valid();
+   requires 0<=key<=|values|
+   ensures Valid();
+   ensures |values|==|old(values)|+1;
+   ensures (values[key]==value);
+   ensures (forall k:: 0<=k<|old(values)| ==> old(values)[k] in values);
+   ensures (forall k:: (k in values <==> k in old(values) || k==value ));
+   ensures (forall k:: (!( k in old(values) || k==value )) ==>(! (k in values)));
+   modifies this;
+   {
+      var tmp_seq:=[value];
+      assert(|tmp_seq|==1);
+      var newValues := values[..key]+tmp_seq[0..|tmp_seq|]+values[key..|values|];
+      assert(|newValues|==|values|+1);
+      assert(0<=key<|newValues|);
+      assert(newValues[key]==value);
+      assert(forall k:: 0<=k<|values| ==> values[k] in newValues);
+      values:=newValues;
+   }
+   
+   
+   
+   method Change(newValues: seq<int>)
+   requires Valid();
+   ensures Valid();
+   modifies this;
+   {
+      values:=newValues;
+   }
+   
+
+}
+
+
+
+
+ this;
+   ensures Valid();
+   ensures |values|==0;
+   {
+      values:=[];
+   }
+   
+   method Length() returns (num:int)
+   requires Valid();
+   ensures Valid();
+   ensures num==|values|
+   {
+      num:=|values|;
+   }
+   
+   method Remove(key:int)
+   requires Valid();
+   ensures Valid();
+   ensures (forall k::0<=k<|old(values)| && k !=key ==> old(values)[k] in values);
+   modifies this;
+   {
+      if(key>=|values| || key <0 |||values|==0){
+         return;
+      }
+      assert(|values|>0&&|values|>key);
+      values := values[..key]+values[(key+1)..|values|];
+      assert(|values|+1==|old(values)|);
+      assert(forall k::0<=k<|old(values)| && k !=key ==> old(values)[k] in values);
+      
+   }
+   
+   
+   
+   method Add(key:int,value:int)
+   requires Valid();
+   requires 0<=key<=|values|
+   ensures Valid();
+   ensures |values|==|old(values)|+1;
+   ensures (values[key]==value);
+   ensures (forall k:: 0<=k<|old(values)| ==> old(values)[k] in values);
+   ensures (forall k:: (k in values <==> k in old(values) || k==value ));
+   ensures (forall k:: (!( k in old(values) || k==value )) ==>(! (k in values)));
+   modifies this;
+   {
+      var tmp_seq:=[value];
+      assert(|tmp_seq|==1);
+      var newValues := values[..key]+tmp_seq[0..|tmp_seq|]+values[key..|values|];
+      assert(|newValues|==|values|+1);
+      assert(0<=key<|newValues|);
+      assert(newValues[key]==value);
+      assert(forall k:: 0<=k<|values| ==> values[k] in newValues);
+      values:=newValues;
+   }
+   
+   
+   
+   method Change(newValues: seq<int>)
+   requires Valid();
+   ensures Valid();
+   modifies this;
+   {
+      values:=newValues;
+   }
+   
+
+}
+
+method discard_by_id (bloodArray: Dynamic_array, id: int) returns (result:bool)
+    requires bloodArray!=null && !(id<0);
+    //All ids need to be unique
+    requires forall k,i:: 0<=k<i< |bloodArray.values| ==> bloodArray.values[i] != bloodArray.values[k]
+    requires id >= 0;
+    ensures result==true ==> (exists k:: 0<=k< old(|bloodArray.values|) && old(bloodArray.values[k]==id))
+    modifies bloodArray;
+{
+    var i := 0;
+    result := false;
+    while (i< |bloodArray.values|)
+    invariant 0<=i<= |bloodArray.values|;
+    invariant result ==true ==> forall k:: 0<=k< |bloodArray.values| ==> bloodArray.values[k]!=id
+    {
+        if (bloodArray.values[i] == id){
+            assert(bloodArray.values[i] == id);
+            result:= true;
+            bloodArray.Remove(i);
+            return;
+        }else{
+            result:= false;
+        }
+        i:=i+1;
+    }
+    return;
+}
+
+
+method discard_all (bloodArray: Dynamic_array, currentDate: int)
+    requires bloodArray!=null && !(currentDate<0);
+    //All ids need to be unique
+    requires forall k,i:: 0<=k<i< |bloodArray.values| ==> bloodArray.values[i] != bloodArray.values[k]
+    requires currentDate >= 0;
+    modifies bloodArray;
+    ensures forall k :: 0<=k<|bloodArray.values| ==> (bloodArray.values[k] >= currentDate)
+    {
+        var i:= 0;
+        var remove := new Dynamic_array();
+        assert(remove!=null);
+        assert(|remove.values|==0);
+        assert(remove.values==[]);
+
+        while (i<|bloodArray.values|)
+        invariant 0<=i<=|bloodArray.values|
+        invariant forall k:: k in remove.values ==> bloodArray.values[k]< currentDate;
+        {
+            //If expires, then add to remove
+            if(bloodArray.values[i] < currentDate){
+                //unshift
+                assert(bloodArray.values[i] < currentDate);
+                remove.Add(0,i);
+                assert(remove.values[0] ==i);
+            }
+            i:= i+1;
+        }
+
+        i:= 0;
+        while (i<|remove.values|)
+        invariant 0<=i<=|remove.values|
+        {
+            bloodArray.Remove(remove.values[i]);
+            i:=i+1;
+        }
+    }
+
+
+method get_all ((bloodArray: Dynamic_array){
+    
 }
